\documentclass[11pt,a4paper]{article}

\input{./conf/usepackage.tex}
\usepackage{chngcntr}

\defaultfontfeatures{Mapping=tex-text}
%\setmainfont{???}
\setdefaultlanguage{german}
\definecolor{114F9D}{HTML}{114F9D}
\author{Zehao Gao}

\input{./conf/newtheorem.tex}
%\renewcommand{\frac}{\dfrac}

\counterwithin*{equation}{section}
%\counterwithin*{equation}{subsection}
%\numberwithin{equation}{section}

\begin{document}

\input{./conf/titlepage.tex}

\newpage

\tableofcontents

\newpage

\input{./Section/1.tex}

\newpage

\input{./Section/2.tex}

\newpage

\input{./Section/3.tex}

\newpage

\input{./Section/4.tex}

\newpage

\input{./Section/5.tex}

\newpage

\input{./Section/6.tex}

\newpage

\input{./Section/7.tex}

\newpage

\input{./Section/8.tex}

\newpage

\input{./Section/9.tex}

\newpage

\input{./Section/10.tex}

\newpage

\input{./Section/11.tex}

\newpage

\input{./Section/12.tex}

\newpage

\input{./Section/13.tex}

\newpage

\input{./Section/14.tex}

\newpage

\input{./Section/15.tex}

\newpage

\input{./Section/16.tex}

\newpage

\input{./Section/17.tex}

\newpage

\input{./Section/18.tex}

\newpage

\input{./Section/19.tex}

\newpage

\input{./Section/20.tex}

\newpage

\input{./Section/21.tex}

\newpage

\section*{Blatt 22}

\newpage

\paragraph{Aufgabe 22.4(H)}

\begin{enumerate}

\item[]

Evaluate the following integral
\begin{align}
\int\frac{1}{x^2-4x+8}dx
&=
\int\frac{1}{(x-2)^2+2^2}dx
\end{align}

substitute $u=\frac{x-2}{2}$, with $du=\frac{1}{2}dx$, we get
\begin{align}
\frac{1}{2}\int\frac{1}{u^2+1}du=\frac{1}{2}\arctan(u)+C=\frac{1}{2}\arctan\bigg(\frac{x-2}{2}\bigg)+C
\end{align}

\end{enumerate}

\paragraph{Aufgabe 22.5(H)}

Calculate antiderivative $F$ of following function $f$.

\begin{enumerate}

\item[(a)]$f(x)=\frac{x^2+9x+17}{x^3+3x^2-4}$

\begin{align}
\frac{x^2+9x+17}{x^3+3x^2-4}=\frac{x^2+9x+17}{(x-1)(x+2)^2}
\end{align}

using partial fraction decomposition
\begin{align}
\frac{x^2+9x+17}{(x-1)(x+2)^2}=\frac{A}{x-1}+\frac{B}{x+2}+\frac{C}{(x+2)^2}
\end{align}

we get
\begin{align}
x^2+9x+17=A(x^2+4x+4)+B(x^2+x-2)+C(x-1)
\end{align}

therefore
\begin{align}
A=3,\hspace{1em}
B=-2,\hspace{1em}
C=-1
\end{align}

then the function $f$ turns to
\begin{align}
f(x)=\frac{3}{x-1}+\frac{-2}{x+2}+\frac{-1}{(x+2)^2}
\end{align}

and the antidderivative is given by
\begin{align}
F(x)=\int f(x)dx
&=\int \frac{3}{x-1}+\frac{-2}{x+2}+\frac{-1}{(x+2)^2}dx \\
&=3\ln(x-1)-2\ln(x+2)+\frac{1}{x+2}+C
\end{align}

\newpage

\item[(b)]$f(x)=\frac{x^4}{x^3+1}$

First we do polynomial long division
\begin{align}
f(x)=\frac{x^4}{x^3+1}=\frac{x(x^3+1)-x}{x^3+1}=x-\frac{x}{x^3+1}=x-\frac{x}{(x+1)(x^2-x+1)}
\end{align}

use partial fraction decomposition
\begin{align}
\frac{x}{x^3+1}=x-\frac{x}{(x+1)(x^2-x+1)}=\frac{A}{x+1}+\frac{Bx+C}{x^2-x+1}
\end{align}
\begin{align}
x=A(x^2-x+1)+(Bx+C)(x+1)
\end{align}

therefore
\begin{align}
A=\frac{-1}{3},\hspace{1em}
B=\frac{1}{3},\hspace{1em}
C=\frac{1}{3}
\end{align}

then we get
\begin{align}
f(x)=x+\frac{1}{3(x+1)}-\frac{x+1}{3(x^2-x+1)}
\end{align}

and
\begin{align}
F(x)=\int f(x)dx
&=\int xdx+\frac{1}{3}\int\frac{1}{x+1}dx-\frac{1}{3}\int\frac{x+1}{x^2-x+1}dx \\
&=\frac{1}{2}x^2+\frac{1}{3}\ln(x+1)+C-\frac{1}{3}
\underset{\mahjong{6z}}{\underbrace{\int\frac{x+1}{x^2-x+1}dx}}
\end{align}

evaluate the following integral
\begin{align}
\mahjong{6z}=\int\frac{x+1}{x^2-x+1}dx
&=\frac{1}{2}\int\frac{2x-1}{x^2-x+1}dx+\frac{3}{2}\int\frac{1}{x^2-x+1}dx \\
&=\frac{1}{2}\ln(x^2-x+1)+C+\frac{3}{2}
\underset{\mahjong{7z}}{\underbrace{\int\frac{1}{x^2-x+1}dx}}
\end{align}

evaluate the following integral
\begin{align}
\mahjong{7z}=\int\frac{1}{x^2-x+1}dx
&=\int\frac{1}{x^2-x+\frac{1}{4}+\frac{3}{4}}dx \\
&=\int\frac{1}{(x-\frac{1}{2})^2+\frac{3}{4}}dx \\
&=\frac{4}{3}\int\frac{1}{\frac{4}{3}(x-\frac{1}{2})^2+1}dx
\end{align}

substitute $u=\frac{2}{\sqrt{3}}(x-\frac{1}{2})$ with $du=\frac{2}{\sqrt{3}}dx$, we get
\begin{align}
\mahjong{7z}=\frac{4}{3}\frac{\sqrt{3}}{2}\int\frac{1}{u^2+1}du=\frac{2\sqrt{3}}{3}\arctan(u)+C=\frac{2\sqrt{3}}{3}\arctan\bigg(\frac{2}{\sqrt{3}}\bigg(x-\frac{1}{2}\bigg)\bigg)+C
\end{align}

\newpage

therefore
\begin{align}
\mahjong{6z}=\frac{1}{2}\ln(x^2-x+1)+\sqrt{3}\arctan\bigg(\frac{2}{\sqrt{3}}\bigg(x-\frac{1}{2}\bigg)\bigg)+C
\end{align}

and we finally get
\begin{align}
F(x)=\frac{1}{2}x^2+\frac{1}{3}\ln(x+1)-\frac{1}{6}\ln(x^2-x+1)-\frac{\sqrt{3}}{3}\arctan\bigg(\frac{2}{\sqrt{3}}\bigg(x-\frac{1}{2}\bigg)\bigg)+C
\end{align}

\end{enumerate}

\vspace*{\fill}
\begin{align*}
\mahjong{123456789p 123456789s 123456789m 1234567z}
\end{align*}

\end{document}