\section*{Blatt 21}

\newpage

\paragraph{Aufgabe 21.5(H)}

Calculate antiderivative of following functions with proper methods:

\begin{enumerate}

\item[(a)]$f(x)=x^3e^x$
\begin{align}
\int f(x)dx
&=\int x^3e^x dx \\
&=x^3e^x-\int 3x^2e^x dx \\
&=x^3e^x-3x^2e^x+\int 6xe^x dx \\
&=x^3e^x-3x^2e^x+6xe^x-\int 6e^x dx \\
&=x^3e^x-3x^2e^x+6xe^x-6e^x+C \\
&=(x^3-3x^2+6x-6)e^x+C
\end{align}\\

\item[(b)]$f(x)=3e^x\sqrt{e^x+1}$

Substitute $t=e^x+1$, therefore
\begin{align}
dt=e^xdx
\end{align}
then we have
\begin{align}
\int f(x)dx=\int 3e^x\sqrt{e^x+1}dx
&=3\int \sqrt{t}dt \\
&=2t^{\sfrac{3}{2}}+C \\
&=2(e^x+1)^{\sfrac{3}{2}}+C
\end{align}
\\

\item[(c)]$f(x)=x\ln x \hspace{1em} (x>0)$
\begin{align}
\int f(x)dx
&=\int x\ln x dx \\
&=\frac{1}{2} \int 2x\ln x dx \\
&=\frac{1}{2}\bigg(x^2\ln x-\int x^2\frac{1}{x}dx\bigg) \\
&=\frac{1}{2}\bigg(x^2\ln x-\frac{1}{2}x^2+C\bigg) \\
&=\frac{x^2}{4}(2\ln x-1)+C
\end{align}

\newpage

\item[(d)]$f(x)=\frac{1}{\sqrt{x}(1+\sqrt[3]{x})} \hspace{1em} (x>0)$
\begin{align}
f(x)
=\frac{1}{\sqrt{x}(1+\sqrt[3]{x})}
=\frac{1}{x^{\sfrac{1}{2}}(1+x^{\sfrac{1}{3}})}
=\frac{1}{x^{\sfrac{1}{2}}+x^{\sfrac{5}{6}}}
=\frac{1}{x^{\sfrac{3}{6}}+x^{\sfrac{5}{6}}}
\end{align}
Substitute $t=x^{\sfrac{1}{6}}$ with $dt=\frac{1}{6x^{\sfrac{5}{6}}}dx$ we get
\begin{align}
\int f(x)dx=\int\frac{1}{x^{\sfrac{3}{6}}+x^{\sfrac{5}{6}}}dx
&=\int\frac{6t^5}{t^3+t^5}dt \\
&=6\int\frac{t^2}{1+t^2}dt \\
&=6\int 1dt-6\int\frac{1}{1+t^2}dt \\
&=6t-6\arctan(t)+C \\
&=6(x^{\sfrac{1}{6}})-6\arctan(x^{\sfrac{1}{6}})+C
\end{align}

\item[(e)]$f(x)=(\ln x)^3$

Substitute $t=\ln x$, with $dt=\frac{1}{x}dx$ and $x=e^t$, we get
\begin{align}
\int f(x)dx=\int (\ln x)^3 dx
&=\int t^3 e^t dt
\end{align}

use the conclusion from (a) eq.1 to 6, we get
\begin{align}
\int t^3 e^t dt=(t^3-3t^2+6t-6)e^t+C
\end{align}

therefore
\begin{align}
\int f(x)dx=(\ln^3 x-3\ln^2 x+6\ln x-6)x+C
\end{align}

\end{enumerate}